\documentclass{article}
\usepackage{amssymb,amsmath}
\begin{document}
\thispagestyle{empty}

\begin{align*}
J(\vec{u}) & = \sum\limits_{i=0}^N \left((x_0-x_N)^2 + 2(x_0-x_N)\sum\limits_{j=0}^{i-1}u_j+\left(\sum\limits_{j=0}^{i-1}u_j\right)^2 + u_i^2\right)\\
& = u_0^2 + 2(x_0-x_N)\sum\limits_{i=0}^N u_0 +  \sum\limits_{i=0}^N u_0^2 + u_0 2 \sum\limits_{i=0}^N \sum\limits_{j=1}^{i-1}u_j + \dots\\
& = u_0^2 + 2N(x_0-x_N) u_0 + N u_0^2 +  u_0  2\sum\limits_{i=0}^N \sum\limits_{j=1}^{i-1}u_j + \dots
\end{align*}
\end{document}


