\documentclass{article}
\usepackage{amssymb,amsmath}
\begin{document}
\thispagestyle{empty}

\begin{align*}
J(\vec{x}_0, U) & = (GU + H\vec{x}_0)^\top\bar{Q}(GU + H\vec{x}_0)+U^\top\bar{R}U=\\
& = U^\top(G^\top\bar{Q}G + \bar{R})U + U^\top G^\top \bar{Q}^\top H\vec{x}_0 + \vec{x}_0^\top H^\top \bar{Q} G U + \vec{x}_0^\top H^\top \bar{Q} H \vec{x}_0 = \\
& = U^\top(G^\top\bar{Q}G + \bar{R})U + 2 \vec{x}_0^\top H^\top \bar{Q} G U + \vec{x}_0^\top H^\top \bar{Q} H \vec{x}_0 
\end{align*}

\end{document}


