\documentclass[A4,11pt]{article}
\usepackage[T2A]{fontenc}
\usepackage[utf8]{inputenc}
\usepackage[russian]{babel}
\usepackage{amsmath,amssymb,amsfonts}
\begin{document}
\thispagestyle{empty}

$$
\{U_j\}_{j=1}^{N}
$$

$$
p(U_j) = \frac{1}{\sqrt{2\pi}\sigma} \exp\left(-\frac{(U_j-U)^2}{2\sigma^2}\right)
$$

\begin{align*}
\log \mathcal{L}(U,\sigma) & = \log \left(\prod\limits_{j=1}^N  \frac{1}{\sqrt{2\pi}\sigma} \exp\left(-\frac{(U_j-U)^2}{2\sigma^2}\right)\right) =\\
& = \sum\limits_{j=1}^N \log \left(\frac{1}{\sqrt{2\pi}\sigma} \exp\left(-\frac{(U_j-U)^2}{2\sigma^2}\right)\right) = \\
& = \sum\limits_{j=1}^N \left(\log \left(\frac{1}{\sqrt{2\pi}\sigma}\right) -\frac{(U_j-U)^2}{2\sigma^2}\right) = \\
& = -N \left(\log\sqrt{2\pi} + \log\sigma\right) - \frac{1}{2\sigma^2} \sum\limits_{j=1}^N (U_j-U)^2
\end{align*}

$$
\frac{\partial\mathcal{L}}{\partial U}    =  \frac{1}{\sigma^2}\sum\limits_{j=1}^N (U_j-U) = 0 
$$

$$
U = \frac{\sum\limits_{j=1}^N U_j}{N}
$$

$$
\frac{\partial\mathcal{L}}{\partial\sigma} =  -\frac{N}{\sigma} + \frac{1}{\sigma^3}\sum\limits_{j=1}^N (U_j-U)^2 = 0
$$

$$
\sigma = \sqrt{\frac{\sum\limits_{j=1}^N (U_j-U)^2}{N}} 
$$

$$
\{I_j, U_j\}_{j=1}^{N}
$$

\begin{align*}
\log \mathcal{L}(R,\sigma) & = \log \left(\prod\limits_{j=1}^N  \frac{1}{\sqrt{2\pi}\sigma} \exp\left(-\frac{(U_j-R I_j)^2}{2\sigma^2}\right)\right) =\\
& = -N \left(\log\sqrt{2\pi} + \log\sigma\right) - \frac{1}{2\sigma^2} \sum\limits_{j=1}^N (U_j- R I_j)^2
\end{align*}

$$
\frac{\partial\mathcal{L}}{\partial R}    =  \frac{1}{\sigma^2}\sum\limits_{j=1}^N (U_j- R I_j) = 0 
$$

$$
R = \frac{\sum\limits_{j=1}^N U_j}{\sum\limits_{j=1}^N I_j}
$$

\end{document}
