\documentclass[A4,11pt]{article}
\usepackage[T2A]{fontenc}
\usepackage[utf8]{inputenc}
\usepackage[russian]{babel}
\usepackage{amsmath,amssymb,amsfonts}
\begin{document}
\thispagestyle{empty}

$$
\left\{
\begin{array}{cccccccc}
a_{11}x_1 & + &  a_{12}x_2  &+      & \cdots & + & a_{1n}x_n &= b_1\\
a_{21}x_1 & + &  a_{22}x_2  &+      & \cdots & + & a_{2n}x_n &= b_2\\
          &   &             &\vdots &        &   &           &     \\
a_{n1}x_1 & + &  a_{n2}x_2  &+      & \cdots & + & a_{nn}x_n &= b_n\\
\end{array}
\right.
$$

\begin{align*}
x_1 &= \frac{1}{a_{11}}(b_1 - a_{12}x_2 - a_{13}x_3 - \cdots - a_{1n}x_n)\\
x_2 &= \frac{1}{a_{22}}(b_2 - a_{21}x_2 - a_{23}x_3 - \cdots - a_{2n}x_n)\\
    & \qquad \vdots \\
x_n &= \frac{1}{a_{nn}}(b_n - a_{n1}x_2 - a_{n2}x_3 - \cdots - a_{n,n-1}x_{n-1})
\end{align*}

$\vec{x}^{(0)}=\left(x_1^{(0)}, x_2^{(0)}, \dots, x_n^{(0)}\right)$

$\vec{x}^{(1)}=\left(x_1^{(1)}, x_2^{(1)}, \dots, x_n^{(1)}\right)$


\begin{align*}
x_1^{(1)} &= \frac{1}{a_{11}}(b_1 - a_{12}x_2^{(0)} - a_{13}x_3^{(0)} - \cdots - a_{1n}x_n^{(0)})\\
x_2^{(1)} &= \frac{1}{a_{22}}(b_2 - a_{21}x_2^{(0)} - a_{23}x_3^{(0)} - \cdots - a_{2n}x_n^{(0)})\\
    & \qquad \vdots \\                                                                          
x_n^{(1)} &= \frac{1}{a_{nn}}(b_n - a_{n1}x_2^{(0)} - a_{n2}x_3^{(0)} - \cdots - a_{n,n-1}x_{n-1}^{(0)})
\end{align*}

$\vec{x}^{(k)}=\left(x_1^{(k)}, x_2^{(k)}, \dots, x_n^{(k)}\right)$

$$
x_i^{(k)} = \frac{1}{a_{ii}} \left(b_i - \sum\limits_{j=1,j\neq i}^n a_{ij}x_j^{(k-1)} \right), \quad \text{for } i=1,2,\dots,n
$$

$$
x_i^{(k)} = \frac{1}{a_{ii}} \left(b_i - \sum\limits_{j=1}^{i-1} a_{ij}x_j^{(k)} -  \sum\limits_{j=i+1}^n a_{ij}x_j^{(k-1)} \right), \quad \text{for } i=1,2,\dots,n
$$

\end{document}
